src/fmap/list_of_pairs.v
@@ -1,0 +1,15 @@
+Require CrossCrypto.fmap.
+Require Import Coq.Lists.List.
+
+Section WithKV.
+  Context {K V : Type}.
+  Context (Keqb : K -> K -> bool).
+  Definition list_of_pairs : @fmap.operations K V :=
+    {|
+      fmap.M := list (K * V);
+      fmap.empty := nil;
+      fmap.add := fun k v => cons (k, v);
+      fmap.find := fun k m => option_map snd (List.find (fun '(k', _) => Keqb k' k) m);
+      fmap.fold_ac := fun S f => List.fold_right (fun '(k, v) => f k v);
+    |}.
+End WithKV.
