src/fmap/list_of_pairs_correct.v
@@ -1,0 +1,12 @@
+Require Import CrossCrypto.fmap.list_of_pairs.
+
+Section WithKV.
+  Context {K V : Type}.
+  Context (Keqb : K -> K -> bool).
+
+  Context (Kper : K -> K -> Prop) (Vper : V -> V -> Prop).
+  (* TODO: require per transitive symmetric *)
+  Context (Keqb_iff : forall k1 k2, Keqb k1 k2 = true <-> Kper k1 k2).
+  Lemma ok : fmap.ok Kper Vper (list_of_pairs Keqb).
+  Abort.
+End WithKV.
