src/fmap.v
@@ -1,0 +1,82 @@
+Section Maps.
+  Local Set Universe Polymorphism.
+  Context {K V : Type}.
+
+  Record operations :=
+    {
+      M : Type;
+      
+      empty : M;
+      add : K -> V -> M -> M;
+      find : K -> M -> option V;
+      (* remove : K -> M V -> M V; *)
+
+      fold_ac : forall S (f : K -> V -> S -> S), S -> M -> S;
+    }.
+
+  Section Spec.
+    Context (Kper : K -> K -> Prop).
+    Context (Vper : V -> V -> Prop).
+    Context (M_operations : operations).
+    Local Notation M := M_operations.(M).
+    Local Notation empty := M_operations.(empty).
+    Local Notation add := M_operations.(add).
+    Local Notation find := M_operations.(find).
+    Local Notation fold_ac := M_operations.(fold_ac).
+
+    Record ok :=
+      {
+        per : M -> M -> Type;
+        ok_empty : per empty empty;
+        ok_add : 
+          forall (k1 k2:K) (_ : Kper k1 k2),
+          forall (v1 v2:V) (_ : Vper v1 v2),
+          forall (m1 m2 : M) (_ : per m1 m2),
+            per (add k1 v1 m1) (add k2 v2 m2);
+        ok_find :
+            forall (k1 k2 : K) (_ : Kper k1 k2),
+            forall (m1 m2 : M) (_ : per m1 m2),
+              (* option_per *)
+              match find k1 m1, find k2 m2 with
+              | Some v1, Some v2 => Vper v1 v2
+              | None, None => True
+              | _, _ => False
+              end;
+        ok_fold_ac :
+                forall S1 S2 (Sper : S1 -> S2 -> Type),
+                forall f1 f2 (_ : forall k1 k2, Kper k1 k2 ->
+                                        forall v1 v2, Vper v1 v2 ->
+                                                  forall s1 s2, Sper s1 s2 ->
+                                                                Sper (f1 k1 v1 s1) (f2 k2 v2 s2)),
+                forall s1 s2 (_ : Sper s1 s2),
+                forall m1 m2 (_ : per m1 m2),
+                  Sper (fold_ac S1 f1 s1 m1) (fold_ac S2 f2 s2 m2);
+
+        find_empty :
+          forall k (_ : Kper k k),
+            match find k empty with
+            | Some _ => False
+            | None => True
+            end;
+        find_add :
+          forall kf (_ : Kper kf kf),
+          forall ka (_ : Kper ka kf),
+          forall va (_ : Vper va va),
+          forall m (_ : per m m),
+            (Kper kf ka -> match find kf (add ka va m) with
+                           | Some vf => Vper vf va
+                           | None => False
+                           end) /\
+            (~ Kper kf ka ->
+             match find kf (add ka va m), find kf m with
+             | Some vf1, Some vf2 => Vper vf1 vf2
+             | None, None => True
+             | _, _ => False
+             end);
+
+        (* TODO: specify fold_ac *)
+      }.
+  End Spec.
+End Maps.
+
+Global Arguments operations : clear implicits.
